src/mapping/PStoRMWThread.v
@@ -1621,4 +1621,15 @@ Module PStoRMWThread.
     - esplits; [|eauto]. etrans; eauto.
     - esplits; [|eauto]. etrans; eauto.
   Qed.
+
+  Variant sim_thread_exec (tid: Ident.t) (n: Time.t) (after_sc: bool)
+    (th_ps: PSThread.t lang_ps) (eu: RMWExecUnit.t (A:=unit)): Prop :=
+    | sim_thread_exec_intro
+        sc eu1 eu2
+        (STEPS1: rtc (RMWExecUnit.state_step None tid) eu eu1)
+        (SIM_THREAD: sim_thread tid n th_ps eu1)
+        (SC: sc = if after_sc then S n else n)
+        (STEPS2: rtc (RMWExecUnit.state_step_dmbsy_over (Some n) sc tid) eu1 eu2)
+        (PROMISES: eu2.(RMWExecUnit.local).(Local.promises) = bot)
+  .
 End PStoRMWThread.
